bound/LowerBound.v
@@ -1782,7 +1782,7 @@ Section PRESERVATION.
               exploit ModSem.midx_none; et. intro T. remember (ModSem.initial_owned_heap x) as X.
               clear HeqX. revert X. rewrite T. i. des_u. ss.
             }
-            intro T. rewrite T. clear T. ss. rewrite in_map_iff in *. des; ss. clarify. ss.
+            intro T. ss. rewrite T. clear T. ss. rewrite in_map_iff in *. des; ss. clarify. ss.
             unfold load_modsems, flip in *. rewrite in_map_iff in *. des; ss. clarify.
             subst prog. rewrite in_map_iff in *. des; clarify.
           }
